More attempts at showing correctness

Correctness.thy
@@ -20,15 +20,14 @@ case False with reds_avoids_live[OF assms(1,2)]
 qed
 
 inductive refines where
-  refinesI: "(\<And> x e S. finite S \<Longrightarrow> (x, e) \<in> set \<Gamma> \<Longrightarrow> x \<in> fdom \<rho> \<Longrightarrow> the (lookup \<rho> x) \<sqsubseteq> \<lbrakk>e\<rbrakk>\<^bsub>fmap_expand \<rho> (fdom \<rho> \<union> S)\<^esub>)
+  refinesI: "heapExtendJoin_cond' \<Gamma> ESem \<rho> \<Longrightarrow> (\<And> x e. (x, e) \<in> set \<Gamma> \<Longrightarrow> x \<in> fdom \<rho> \<Longrightarrow> the (lookup \<rho> x) \<sqsubseteq> \<lbrakk>e\<rbrakk>\<^bsub>\<lbrace>\<Gamma>\<rbrace>\<rho>\<^esub>)
       \<Longrightarrow> refines \<Gamma> \<rho>"
 
 lemma refinesD:
   assumes "refines \<Gamma> \<rho>"
-  assumes "finite S"
   assumes "(x, e) \<in> set \<Gamma>"
   assumes "x \<in> fdom \<rho>"
-  shows "the (lookup \<rho> x) \<sqsubseteq> \<lbrakk>e\<rbrakk>\<^bsub>fmap_expand \<rho> (fdom \<rho> \<union> S)\<^esub>"
+  shows "the (lookup \<rho> x) \<sqsubseteq> \<lbrakk>e\<rbrakk>\<^bsub>\<lbrace>\<Gamma>\<rbrace>\<rho>\<^esub>"
 using assms
  by (metis refines.simps)
 
@@ -37,59 +36,18 @@ lemma refinesD':
   assumes "finite S"
   assumes "(x, e) \<in> set \<Gamma>"
   assumes "x \<in> fdom \<rho> \<union> S"
-  shows "the (lookup (fmap_expand \<rho> (fdom \<rho> \<union> S)) x) \<sqsubseteq> \<lbrakk>e\<rbrakk>\<^bsub>fmap_expand \<rho> (fdom \<rho> \<union> S)\<^esub>"
+  shows "the (lookup (fmap_expand \<rho> (fdom \<rho> \<union> S)) x) \<sqsubseteq> \<lbrakk>e\<rbrakk>\<^bsub>\<lbrace>\<Gamma>\<rbrace>\<rho>\<^esub>"
   using assms
   apply (cases "x \<in> fdom \<rho>")
   apply (auto dest: refinesD)
   done
 
-lemma refines_subsetD:
-  "refines \<Gamma> \<rho> \<Longrightarrow> set \<Delta> \<subseteq> set \<Gamma> \<Longrightarrow> refines \<Delta> \<rho>"
-  apply (rule refinesI)
-  apply (frule (1) subsetD)
-  apply (drule (3) refinesD)
-  apply assumption
-  done
-
-lemma refines_insertI:
-  assumes "refines \<Gamma> \<rho>"
-  assumes "\<And> S. finite S \<Longrightarrow> x \<in> fdom \<rho> \<Longrightarrow> the (lookup \<rho> x) \<sqsubseteq> \<lbrakk>e\<rbrakk>\<^bsub>fmap_expand \<rho> (fdom \<rho> \<union> S)\<^esub>"
-  shows "refines ((x,e) # \<Gamma>) \<rho>"
-proof(rule refinesI)
-  case (goal1 x' e' S)
-  note `finite S`[simp]
-  show ?case
-  proof(cases "(x', e') = (x, e)")
-  case True
-    with goal1 have "x \<in> fdom \<rho>" by auto
-    from assms(2)[OF goal1(1) this]
-    show ?thesis using True by simp
-  next
-  case False
-    hence "(x', e') \<in> set \<Gamma>" using goal1(2) by auto
-    from refinesD[OF assms(1) goal1(1) this goal1(3)]
-    show ?thesis
-      apply (rule below_trans)
-      apply (rule ESem_mono_fdom_changes)
-      apply (subst fmap_expand_idem)
-      apply auto
-      done
-  qed
-qed
-
-lemma compatible_fmap_expand:
-  assumes "\<And> x. x \<in> fdom \<rho>1 \<Longrightarrow> x \<in> fdom \<rho>2 \<Longrightarrow> compatible (the (lookup \<rho>1 x)) (the (lookup \<rho>2 x))"
-  shows "compatible (fmap_expand \<rho>1 S) (fmap_expand \<rho>2 S)"
-  apply (case_tac "finite S")
-  apply (rule compatible_fmap_is_compatible[OF compatible_fmapI])
-  apply (case_tac "x \<in> fdom \<rho>1")
-  apply (case_tac "x \<in> fdom \<rho>2")
-  apply (auto simp add: assms fmap_expand_nonfinite)
-  done
-
 lemma refines_is_heapExtendJoin_cond:
   assumes "refines \<Gamma> \<rho>"
   shows "heapExtendJoin_cond' \<Gamma> ESem \<rho>" (is "fix_on_cond_jfc' ?\<rho> ?F")
+  using assms
+ by (metis refines.simps)
+(*
 proof (rule fix_on_cond_jfc'I[OF cont_compose[OF fmap_expand_cont cont2cont_heapToEnv[OF ESem_cont]]])
   fix i
   have compat: "compatible ?\<rho> (?F ?\<rho>)"
@@ -124,6 +82,56 @@ proof (rule fix_on_cond_jfc'I[OF cont_compose[OF fmap_expand_cont cont2cont_heap
     done
   qed
 qed
+*)
+
+(*
+lemma refines_subsetD:
+  "refines \<Gamma> \<rho> \<Longrightarrow> set \<Delta> \<subseteq> set \<Gamma> \<Longrightarrow> refines \<Delta> \<rho>"
+  apply (rule refinesI)
+  apply (drule refines_is_heapExtendJoin_cond)
+  apply (frule (1) subsetD)
+  apply (drule (3) refinesD)
+  apply assumption
+  done
+*)
+
+
+lemma refines_insertI:
+  assumes "refines \<Gamma> \<rho>"
+  assumes "heapExtendJoin_cond' ((x, e) # \<Gamma>) ESem \<rho>"
+  assumes "x \<in> fdom \<rho> \<Longrightarrow> the (lookup \<rho> x) \<sqsubseteq> \<lbrakk>e\<rbrakk>\<^bsub>\<lbrace>(x,e) # \<Gamma>\<rbrace>\<rho>\<^esub>"
+  shows "refines ((x,e) # \<Gamma>) \<rho>"
+proof(rule refinesI[OF assms(2)])
+  case (goal1 x' e')
+  show ?case
+  proof(cases "(x', e') = (x, e)")
+  case True
+    with goal1 have "x \<in> fdom \<rho>" by auto
+    from assms(3)[OF this]
+    show ?thesis using True by simp
+  next
+  case False
+    hence "(x', e') \<in> set \<Gamma>" using goal1(1) by auto
+    from refinesD[OF assms(1) this goal1(2)]
+    show ?thesis
+      apply (rule below_trans)
+      apply (rule cont2monofunE[OF ESem_cont])
+      sorry
+(*    apply (rule HSem_mono_subset)
+      apply auto
+      done *)
+  qed
+qed
+
+lemma compatible_fmap_expand:
+  assumes "\<And> x. x \<in> fdom \<rho>1 \<Longrightarrow> x \<in> fdom \<rho>2 \<Longrightarrow> compatible (the (lookup \<rho>1 x)) (the (lookup \<rho>2 x))"
+  shows "compatible (fmap_expand \<rho>1 S) (fmap_expand \<rho>2 S)"
+  apply (case_tac "finite S")
+  apply (rule compatible_fmap_is_compatible[OF compatible_fmapI])
+  apply (case_tac "x \<in> fdom \<rho>1")
+  apply (case_tac "x \<in> fdom \<rho>2")
+  apply (auto simp add: assms fmap_expand_nonfinite)
+  done
 
 
 theorem correctness:
@@ -172,27 +180,29 @@ case (Variable x e \<Gamma> L \<Delta> z \<rho>)
     by (rule reds_avoids_live[OF `removeAll (x, e) \<Gamma> : e \<Down>\<^bsub>x#L\<^esub> \<Delta> : z`, unfolded heapVars_def, rotated], simp)
 
   assume "refines \<Gamma> \<rho>"
-  hence "refines (removeAll (x, e) \<Gamma>) \<rho>" by (auto intro: refines_subsetD)
+  hence "refines (removeAll (x, e) \<Gamma>) \<rho>" sorry (* by (auto intro: refines_subsetD) *)
   assume "fdom \<rho> \<subseteq> set L" 
   hence "fdom \<rho> \<subseteq> set (x # L)" by (metis set_subset_Cons subset_trans)
 
   note hyps = Variable.hyps(3-5)[OF `refines (removeAll (x, e) \<Gamma>) \<rho>` `fdom \<rho> \<subseteq> set (x#L)`]
 
-  thm refinesD[OF `refines \<Gamma> \<rho>` _ `(x,e) \<in> set \<Gamma>`]
+  thm refinesD[OF `refines \<Gamma> \<rho>` `(x,e) \<in> set \<Gamma>`]
 
   from `refines \<Delta> \<rho>`
   have "refines ((x, z) # \<Delta>) \<rho>"
+    (*
     apply (rule refines_insertI)
     apply (rule below_trans)
     apply (erule (1) refinesD[OF `refines \<Gamma> \<rho>` _ `(x,e) \<in> set \<Gamma>`])
     find_theorems e z
+    *)
   sorry
 
   have cond: "heapExtendJoin_cond' \<Gamma> ESem \<rho>"
     by (rule refines_is_heapExtendJoin_cond, fact)
 
   have cond: "heapExtendJoin_cond' ((x, e) # removeAll (x, e) \<Gamma>) ESem \<rho>"
-    (* simple consequence of set being equals *)
+    (* simple consequence of set being equal *)
     sorry
   have cond2: "heapExtendJoin_cond' ((x, z) # \<Delta>) ESem \<rho>"
     by (rule refines_is_heapExtendJoin_cond, fact)
@@ -263,9 +273,8 @@ case (Variable x e \<Gamma> L \<Delta> z \<rho>)
     apply auto
     apply (rule larger_is_join)
     apply (cases "x \<in> fdom \<rho>")
-    apply (rule below_trans[OF refinesD'[OF `refines ((x, z) # \<Delta>) \<rho>`, of "fst ` set  ((x, z) # \<Delta>)", simplified]])
+    apply (rule refinesD'[OF `refines ((x, z) # \<Delta>) \<rho>`, of "fst ` set  ((x, z) # \<Delta>)", simplified])
     apply auto[2]
-    apply (rule cont2monofunE[OF ESem_cont HSem_refines[OF cond2, simplified]])
     apply simp
     done
   finally show ?case.
